Invariant/ValidAttacker/ValidAttackerI/BruteForce.v
@@ -1,0 +1,129 @@
+Require Import Coq.Lists.List.
+
+Require Import Machine.Machine.
+Require Import Machine.MachineValid.
+Require Import Machine.MachineAuxFunctions.
+Require Import Attacker.Attacker.
+Require Import Technique.Technique.
+Require Import Technique.TechniquePreCondition.
+Require Import Technique.TechniquePostCondition.
+
+Require Import Invariant.AuxLemmas.AuxLemmasEnviroment.
+Require Import Invariant.AuxLemmas.AuxLemmasAccount.
+Require Import Invariant.AuxTactics.
+
+Lemma one_step_brute_force_preserves_valid_attacker_i : forall (a a' : Attacker) (n: network_map) (aValid: valid_attacker a n) (m m': idMachine) (u u': idUser) (s': idService),
+      valid_concrete_network n -> Pre a (Brute_Force m u m' u' s') -> Post a (Brute_Force m u m' u' s') n a' -> valid_attacker_i a'.
+  Proof.
+    intros a a' network validAttacker m m' u u' s' validNetwork pre post.
+    unfold valid_attacker_i.
+    intros m0 u0 H_known_machines_a'.
+    unfold valid_attacker in validAttacker.
+    elim_intro_clear validAttacker validAttackerI validAttacker'.
+    unfold Pre in pre; unfold Post in post.
+
+    elim_intro_clear post known_machines_eq post'.
+    elim_intro_clear post' secrets_eq post.
+    elim_intro_clear post exploits_eq post'.
+    elim_intro_clear post' mac post.
+    elim_intro_clear post macView' post'.
+    elim_intro_clear post' newMacView post.
+    elim_intro_clear post accs post'.
+    elim_intro_clear post' accsView' post.
+    elim_intro_clear post newAccountsView post'.
+    elim_intro_clear post' acc post.
+    elim_intro_clear post k post'.
+    elim_intro_clear post' l post.
+    elim_intro_clear post env_m' post'.
+    elim_intro_clear post' network_m' post.
+    elim_intro_clear post accsView'_eq post'.
+    elim_intro_clear post' accs_eq post.
+    elim_intro_clear post acc_in post'.
+    elim_intro_clear post' acc_user post.
+    elim_intro_clear post acc_service post'.
+    elim_intro_clear post' acc_key post.
+    elim_intro_clear post acc_priv post'.
+    elim_intro_clear post' newAccountsView_eq post.
+    elim_intro_clear post newMacView_eq env_a'.
+
+    unfold valid_attacker_i in validAttackerI.
+    rewrite known_machines_eq in H_known_machines_a'.
+
+    case (idMachine_eq m0 m'); case (idUser_eq u0 u'); intros.
+    - unfold modify_machine in env_a'.
+      rewrite env_a'.
+      case (idMachine_eq m0 m'); intro.
+      -- exists newMacView.
+         split.
+         --- reflexivity.
+         --- unfold registered_users.
+             exists acc.
+             split.
+             ---- rewrite acc_user.
+                  symmetry.
+                  exact e.
+             ---- rewrite newMacView_eq.
+                  simpl.
+                  rewrite newAccountsView_eq.
+                  apply member_addAccount.
+                  auto.
+      -- contradiction.
+    
+   - elim (validAttackerI m0 u0).
+      intros MAC IH.
+      elim_intro_clear IH env_MAC users_MAC.
+      -- exists newMacView.
+         split.
+         --- rewrite env_a'.
+             unfold modify_machine.
+             case (idMachine_eq m0 m'); intro eq_m.
+             ---- reflexivity.
+             ---- contradiction.
+         --- unfold registered_users.
+             rewrite newMacView_eq.
+             simpl.
+             rewrite newAccountsView_eq.
+             rewrite e in env_MAC.
+             assert (macView' = MAC).
+             {
+               apply (enviroment_map_image (enviroment a) m' macView' MAC).
+               - exact env_m'.
+               - exact env_MAC.
+             }
+             
+             ---- unfold registered_users in users_MAC.
+                  rewrite <- H in users_MAC.
+                  elim_intro_clear users_MAC acc_u0 users_MAC'.
+                  elim_intro_clear users_MAC' acc_u0_eq acc_In_accounts.
+                  exists acc_u0.
+                  split.
+                  ----- exact acc_u0_eq.
+                  ----- apply addAccount_preserves_membership_when_neq.
+                        ------- rewrite acc_u0_eq.
+                                rewrite acc_user.
+                                exact n.
+                        ------- rewrite <- accsView'_eq. exact acc_In_accounts.
+      -- exact H_known_machines_a'.
+    - elim (validAttackerI m0 u0).
+      intros MAC IH.
+      elim_intro_clear IH env_MAC users_MAC.
+      exists MAC.
+      split.
+      -- rewrite (enviroment_eq (enviroment a) (enviroment a') m0 m' newMacView).
+         --- exact env_MAC.
+         --- exact n.
+         --- exact env_a'.
+      -- exact users_MAC.
+      -- exact H_known_machines_a'.
+    - elim (validAttackerI m0 u0).
+      intros MAC IH.
+      elim_intro_clear IH env_MAC users_MAC.
+      exists MAC.
+      split.
+      -- rewrite (enviroment_eq (enviroment a) (enviroment a') m0 m' newMacView).
+         --- exact env_MAC.
+         --- exact n0.
+         --- exact env_a'.
+      -- exact users_MAC.
+      -- exact H_known_machines_a'.
+  Qed.
