Invariant/ValidAttacker/ValidAttackerII/BruteForce.v
@@ -1,0 +1,81 @@
+Require Import Coq.Lists.List.
+
+Require Import Machine.Machine.
+Require Import Machine.MachineValid.
+Require Import Machine.MachineAuxFunctions.
+Require Import Attacker.Attacker.
+Require Import Technique.Technique.
+Require Import Technique.TechniquePreCondition.
+Require Import Technique.TechniquePostCondition.
+
+Require Import Invariant.AuxLemmas.AuxLemmasEnviroment.
+Require Import Invariant.AuxLemmas.AuxLemmasAccount.
+Require Import Invariant.AuxTactics.
+
+Lemma one_step_brute_force_preserves_valid_attacker_ii : forall (a a' : Attacker) (n: network_map) (aValid: valid_attacker a n) (m m': idMachine) (u u': idUser) (s': idService),
+      valid_concrete_network n -> Pre a (Brute_Force m u m' u' s') -> Post a (Brute_Force m u m' u' s') n a' -> valid_attacker_ii a'.
+  Proof.
+    intros a a' network validAttacker m m' u u' s' validNetwork pre post.
+    unfold valid_attacker_ii.
+    intros m0 p0 H_secrets_a'.
+    unfold valid_attacker in validAttacker.
+    elim_intro_clear validAttacker validAttackerI validAttacker'.
+    elim_intro_clear validAttacker' validAttackerII validAttacker.
+    unfold Pre in pre; unfold Post in post.
+
+    elim_intro_clear post known_machines_eq post'.
+    elim_intro_clear post' secrets_eq post.
+    elim_intro_clear post exploits_eq post'.
+    elim_intro_clear post' mac post.
+    elim_intro_clear post macView' post'.
+    elim_intro_clear post' newMacView post.
+    elim_intro_clear post accs post'.
+    elim_intro_clear post' accsView' post.
+    elim_intro_clear post newAccountsView post'.
+    elim_intro_clear post' acc post.
+    elim_intro_clear post k post'.
+    elim_intro_clear post' l post.
+    elim_intro_clear post env_m' post'.
+    elim_intro_clear post' network_m' post.
+    elim_intro_clear post accsView'_eq post'.
+    elim_intro_clear post' accs_eq post.
+    elim_intro_clear post acc_in post'.
+    elim_intro_clear post' acc_user post.
+    elim_intro_clear post acc_service post'.
+    elim_intro_clear post' acc_key post.
+    elim_intro_clear post acc_priv post'.
+    elim_intro_clear post' newAccountsView_eq post.
+    elim_intro_clear post newMacView_eq env_a'.
+
+    unfold valid_attacker_ii in validAttackerII.
+    elim (validAttackerII m0 p0).
+    intros MAC IH.
+    elim_intro_clear IH env_MAC path_MAC.
+    - case (idMachine_eq m0 m'); intro eq_m0.
+      -- exists newMacView.
+         split.
+         --- rewrite env_a'.
+             unfold modify_machine.
+             case (idMachine_eq m0 m'); intros.
+             ---- reflexivity.
+             ---- contradiction.
+         --- unfold registered_paths.
+             rewrite newMacView_eq.
+             simpl.
+             assert (macView' = MAC).
+             ---- apply (enviroment_map_image (enviroment a) m' macView' MAC).
+                  ----- exact env_m'.
+                  ----- rewrite <- eq_m0. exact env_MAC.
+             ---- unfold registered_paths in path_MAC.
+                  rewrite <- H in path_MAC.
+                  exact path_MAC.
+      -- exists MAC.
+         rewrite (enviroment_eq (enviroment a) (enviroment a') m0 m' newMacView).
+         --- split.
+             ---- exact env_MAC.
+             ---- exact path_MAC.
+         --- exact eq_m0.
+         --- exact env_a'.
+    - rewrite secrets_eq in H_secrets_a'.
+      exact H_secrets_a'.
+  Qed.
