Invariant/ValidAttacker/ValidAttackerIII/AccountDiscoveryLocal.v
@@ -1,0 +1,142 @@
+Require Import Coq.Lists.List.
+
+Require Import Machine.Machine.
+Require Import Machine.MachineValid.
+Require Import Machine.MachineAuxFunctions.
+Require Import Attacker.Attacker.
+Require Import Technique.Technique.
+Require Import Technique.TechniquePreCondition.
+Require Import Technique.TechniquePostCondition.
+
+Require Import Invariant.AuxLemmas.AuxLemmasEnviroment.
+Require Import Invariant.AuxLemmas.AuxLemmasAccount.
+Require Import Invariant.AuxTactics.
+
+Lemma one_step_account_discovery_local_preserves_valid_attacker_iii : forall (a a' : Attacker) (n: network_map) (aValid: valid_attacker a n) (m : idMachine) (u : idUser) (s: idService),
+      valid_concrete_network n -> Pre a (Account_Discovery_Local m u s) -> Post a (Account_Discovery_Local m u s) n a' -> valid_attacker_iii a'.
+  Proof.
+    intros a a' network validAttacker m u s validNetwork pre post.
+    unfold valid_attacker_iii.
+    unfold valid_network.
+    elim_intro_clear validAttacker validAttackerI validAttacker'.
+    elim_intro_clear validAttacker' validAttackerII validAttacker''.
+    elim_intro_clear validAttacker'' validAttackerIII validAttackerIV.
+    unfold Pre in pre; unfold Post in post.
+
+    elim_intro_clear post known_machines_eq post'.
+    elim_intro_clear post' secrets_eq post.
+    elim_intro_clear post mastered_exploits_eq post'.
+    elim_intro_clear post' mac post.
+    elim_intro_clear post macView post'.
+    elim_intro_clear post' newMacView post.
+    elim_intro_clear post accs post'.
+    elim_intro_clear post' accsView post.
+    elim_intro_clear post newAccountsView post'.
+    elim_intro_clear post' accsLinkedToService post.
+    elim_intro_clear post env_m post'.
+    elim_intro_clear post' network_m post.
+    elim_intro_clear post accs_eq post'.
+    elim_intro_clear post' accsView_eq post.
+    elim_intro_clear post accsLinkedToService_eq post'.
+    elim_intro_clear post' newAccountsView_eq post.
+    elim_intro_clear post newMacView_eq env_a'.
+
+    unfold valid_attacker_iii in validAttackerIII.
+    unfold valid_network in validAttackerIII.
+    elim_intro_clear validAttackerIII network_top_enva valid_machine_enva.
+    unfold network_topology in *.
+    split.
+    - intros.
+      rewrite env_a'.
+      unfold modify_machine.
+      case (idMachine_eq neighbour m); case (idMachine_eq mid m); intros eq_mid eq_neigh.
+      -- exists newMacView; auto.
+      -- exists newMacView; auto.
+      -- apply (network_top_enva m neighbour macView).
+         --- intro contra. symmetry in contra. exact (eq_neigh contra).
+         --- exact env_m.
+         --- assert (m0 = newMacView).
+             ---- apply (enviroment_simpl (enviroment a) (enviroment a') mid m).
+                  ----- exact eq_mid.
+                  ----- exact env_a'.
+                  ----- exact H0.
+             ---- rewrite H2 in H1.
+                  rewrite newMacView_eq in H1.
+                  unfold is_neighbour in *.
+                  simpl in H1.
+                  exact H1.
+      -- apply (network_top_enva mid neighbour m0).
+         --- exact H.
+         --- rewrite <- (enviroment_eq (enviroment a) (enviroment a') mid m newMacView).
+             ---- exact H0.
+             ---- exact eq_mid.
+             ---- exact env_a'.
+         --- exact H1.
+    - intros.
+      case (idMachine_eq mid m); intros eq_m.
+      -- assert (m0 = newMacView).
+         apply (enviroment_simpl (enviroment a) (enviroment a') mid m).
+         --- exact eq_m.
+         --- exact env_a'.
+         --- exact H.
+         --- rewrite H0.
+             elim (valid_machine_enva m macView).
+             intros.
+             elim_intro_clear H2 H3 H2'.
+             elim_intro_clear H2' H4 H5.
+             unfold valid_machine.
+             rewrite newMacView_eq.
+             split.
+             ---- unfold users_access_to_files in *.
+                  unfold registered_users in *.
+                  simpl.
+                  rewrite newAccountsView_eq.
+                  intros f Hinf.
+                  destruct (H1 f Hinf) as [Hacc_user H6].
+                  destruct H6 as [ Hacc Hin_f].
+                  destruct Hacc as [acc0 Hacc'].
+                  destruct Hacc' as [ Heq_acc Hin_acc ].
+                  exists Hacc_user.
+                  split.
+                  ----- apply oplusAccounts_preserves_registered_user.
+                        exists acc0.
+                        split.
+                        ------ exact Heq_acc.
+                        ------ rewrite accsView_eq. exact Hin_acc.
+                  ----- exact Hin_f.
+             ---- split.
+                  ----- unfold users_access_to_services in *.
+                        unfold registered_service in *.
+                        rewrite newAccountsView_eq.
+                        simpl.
+                        intros acc0 HIP.
+                        apply member_oplusAccounts_simpl in HIP.
+                        destruct HIP as [Hin_linked | Hin_view].
+                        ------ right.
+                               rewrite accsLinkedToService_eq in Hin_linked.
+                               pose proof (get_accounts_linked_service_without_key_service u s accs acc0 Hin_linked) as Hserv_acc0.
+                               exists s. split.
+                               ------- exact Hserv_acc0.
+                               ------- destruct pre as [_ pre_exists].
+                                       destruct pre_exists as [mac_pre [serv_pre [acc_pre [k_pre [l_pre Hpre_body]]]]].
+                                       destruct Hpre_body as [env_m_pre [Hin_serv [Hval_serv _]]].
+                                       pose proof (enviroment_map_image (enviroment a) m macView mac_pre env_m env_m_pre) as Hmac_eq.
+                                       exists serv_pre. split.
+                                       -------- exact Hval_serv.
+                                       -------- rewrite Hmac_eq. exact Hin_serv.
+                        ------ rewrite accsView_eq in Hin_view.
+                               exact (H3 acc0 Hin_view).
+                  ----- unfold valid_fileSystem.
+                        simpl.
+                        split.
+                        ------ exact H4.
+                        ------ exact H5.
+             ---- exact env_m.
+      -- assert (enviroment a' mid = enviroment a mid).
+         apply (enviroment_eq (enviroment a) (enviroment a') mid m newMacView).
+         --- exact eq_m.
+         --- exact env_a'.
+         --- rewrite H0 in H.
+             apply (valid_machine_enva mid m0).
+             exact H.
+  Qed.
