Invariant/ValidAttacker/ValidAttackerIII/BruteForce.v
@@ -1,0 +1,166 @@
+Require Import Coq.Lists.List.
+
+Require Import Machine.Machine.
+Require Import Machine.MachineValid.
+Require Import Machine.MachineAuxFunctions.
+Require Import Attacker.Attacker.
+Require Import Technique.Technique.
+Require Import Technique.TechniquePreCondition.
+Require Import Technique.TechniquePostCondition.
+
+Require Import Invariant.AuxLemmas.AuxLemmasEnviroment.
+Require Import Invariant.AuxLemmas.AuxLemmasAccount.
+Require Import Invariant.AuxTactics.
+
+Lemma one_step_brute_force_preserves_valid_attacker_iii : forall (a a' : Attacker) (n: network_map) (aValid: valid_attacker a n) (m m': idMachine) (u u': idUser) (s': idService),
+      valid_concrete_network n -> Pre a (Brute_Force m u m' u' s') -> Post a (Brute_Force m u m' u' s') n a' -> valid_attacker_iii a'.
+  Proof.
+    intros a a' network validAttacker m m' u u' s' validNetwork pre post.
+    unfold valid_attacker_iii.
+    unfold valid_network.
+    elim_intro_clear validAttacker validAttackerI validAttacker'.
+    elim_intro_clear validAttacker' validAttackerII validAttacker''.
+    elim_intro_clear validAttacker'' validAttackerIII validAttackerIV.
+    unfold Pre in pre; unfold Post in post.
+
+    elim_intro_clear post known_machines_eq post'.
+    elim_intro_clear post' secrets_eq post.
+    elim_intro_clear post exploits_eq post'.
+    elim_intro_clear post' mac post.
+    elim_intro_clear post macView' post'.
+    elim_intro_clear post' newMacView post.
+    elim_intro_clear post accs post'.
+    elim_intro_clear post' accsView' post.
+    elim_intro_clear post newAccountsView post'.
+    elim_intro_clear post' acc post.
+    elim_intro_clear post k post'.
+    elim_intro_clear post' l post.
+    elim_intro_clear post env_m' post'.
+    elim_intro_clear post' network_m' post.
+    elim_intro_clear post accsView'_eq post'.
+    elim_intro_clear post' accs_eq post.
+    elim_intro_clear post acc_in post'.
+    elim_intro_clear post' acc_user post.
+    elim_intro_clear post acc_service post'.
+    elim_intro_clear post' acc_key post.
+    elim_intro_clear post acc_priv post'.
+    elim_intro_clear post' newAccountsView_eq post.
+    elim_intro_clear post newMacView_eq env_a'.
+
+    unfold valid_attacker_iii in validAttackerIII.
+    unfold valid_network in validAttackerIII.
+    elim_intro_clear validAttackerIII network_top_enva valid_machine_enva.
+    unfold network_topology in *.
+    split.
+    - intros.
+      rewrite env_a'.
+      unfold modify_machine.
+      case (idMachine_eq neighbour m'); case (idMachine_eq mid m'); intros eq_mid eq_neigh.
+      -- exists newMacView; auto.
+      -- exists newMacView; auto.
+      -- apply (network_top_enva m' neighbour macView').
+         --- intro contra. symmetry in contra. exact (eq_neigh contra).
+         --- exact env_m'.
+         --- assert (m0 = newMacView).
+             ---- apply (enviroment_simpl (enviroment a) (enviroment a') mid m').
+                  ----- exact eq_mid.
+                  ----- exact env_a'.
+                  ----- exact H0.
+             ---- rewrite H2 in H1.
+                  rewrite newMacView_eq in H1.
+                  unfold is_neighbour in *.
+                  simpl in H1.
+                  exact H1.
+      -- apply (network_top_enva mid neighbour m0).
+         --- exact H.
+         --- rewrite <- (enviroment_eq (enviroment a) (enviroment a') mid m' newMacView).
+             ---- exact H0.
+             ---- exact eq_mid.
+             ---- exact env_a'.
+         --- exact H1.
+    - intros.
+      case (idMachine_eq mid m'); intros eq_m.
+      -- assert (m0 = newMacView).
+         apply (enviroment_simpl (enviroment a) (enviroment a') mid m').
+         --- exact eq_m.
+         --- exact env_a'.
+         --- exact H.
+         --- rewrite H0.
+             elim (valid_machine_enva m' macView').
+             intros.
+             elim_intro_clear H2 H3 H2'.
+             elim_intro_clear H2' H4 H5.
+             unfold valid_machine.
+             rewrite newMacView_eq.
+             split.
+             ---- unfold users_access_to_files in *.
+                  unfold registered_users in *.
+                  simpl.
+                  rewrite newAccountsView_eq.
+                  intros f Hinf.
+                  destruct (H1 f Hinf) as [Hacc_user H6].
+                  destruct H6 as [ Hacc Hin_f].
+                  destruct Hacc as [acc0 Hacc'].
+                  destruct Hacc' as [ Heq_acc Hin_acc ].
+                  case (idUser_eq Hacc_user u'); intros Heq_u0.
+                  ----- exists Hacc_user.
+                        split.
+                        ------ exists acc.
+                              split.
+                              ------- rewrite acc_user. symmetry. exact Heq_u0.
+                              ------- apply member_addAccount. auto.
+                        ------ exact Hin_f.
+                  ----- exists Hacc_user.
+                        split.
+                        ------ exists acc0.
+                              split.
+                              ------- exact Heq_acc.
+                              ------- apply addAccount_preserves_membership_when_neq.
+                                    -------- rewrite Heq_acc. rewrite acc_user. exact Heq_u0.
+                                    -------- rewrite <- accsView'_eq. exact Hin_acc.
+                        ------ exact Hin_f.
+             ---- split.
+                  ----- unfold users_access_to_services in *.
+                        unfold registered_service in *.
+                        rewrite newAccountsView_eq.
+                        simpl.
+                        intros acc0 HIP.
+                        apply member_addAccount_simpl in HIP.
+                        elim HIP; intro HIP'.
+                        ------ (* HIP' : acc = acc0 *)
+                               right.
+                               rewrite <- HIP'.
+                               exists s'.
+                               split.
+                               ------- exact acc_service.
+                               ------- destruct pre as [_ [_ [accP [macP [lP [env_m'_pre [accP_in [_ [accP_service [_ _]]]]]]]]]].
+                                       assert (Hmac_eq: macP = macView').
+                                       { 
+                                          apply (enviroment_map_image (enviroment a) m' macP macView').
+                                          - exact env_m'_pre.
+                                          - exact env_m'. 
+                                       }
+                                       rewrite Hmac_eq in accP_in.
+                                       destruct (H3 accP accP_in) as [Hnone | [s0 [Hs0 Hserv]]].
+                                       -------- rewrite accP_service in Hnone. discriminate.
+                                       -------- rewrite accP_service in Hs0.
+                                                injection Hs0 as Hs0.
+                                                rewrite <- Hs0 in Hserv.
+                                                exact Hserv.
+                        ------ apply H3.
+                               rewrite <- accsView'_eq in HIP'.
+                               exact HIP'.
+                  ----- unfold valid_fileSystem.
+                        simpl.
+                        split.
+                        ------ exact H4.
+                        ------ exact H5.
+             ---- exact env_m'.
+      -- assert (enviroment a' mid = enviroment a mid).
+         apply (enviroment_eq (enviroment a) (enviroment a') mid m' newMacView).
+         --- exact eq_m.
+         --- exact env_a'.
+         --- rewrite H0 in H.
+             apply (valid_machine_enva mid m0).
+             exact H.
+  Qed.
